* Changes semantic of "and" in definition. Operands don't have a side effect anymore. * Comments out some proofs & fixes type errors. * Introduces xgrd_in

lean/src/defs.lean
@@ -43,18 +43,18 @@ inductive Gdt
 inductive Result
 | leaf (leaf: Leaf) : Result
 | diverged : Result
-| no_match (env: Env) : Result
+| no_match : Result
 
 def gdt_eval : Gdt → Env → Result
 | (Gdt.leaf leaf) env := Result.leaf leaf
 | (Gdt.branch tr1 tr2) env :=
     match gdt_eval tr1 env with
-    | Result.no_match env := gdt_eval tr2 env
+    | Result.no_match := gdt_eval tr2 env
     | r := r
     end
 | (Gdt.grd (Grd.xgrd grd) tr) env :=
     match xgrd_eval grd env with
-    | none := Result.no_match env
+    | none := Result.no_match
     | some val := gdt_eval tr val
     end
 -- This is the only new case
@@ -63,25 +63,30 @@ def gdt_eval : Gdt → Env → Result
     then Result.diverged
     else gdt_eval tr env
 
+
 -- # Refinement Types
 
 -- ## Syntax
 inductive Φ
 | false : Φ
 | true : Φ
-| xgrd (xgrd: XGrd) : Φ
+| xgrd_in (xgrd: XGrd) (ty: Φ) : Φ
 | not_xgrd (xgrd: XGrd) : Φ
-| var_is_bottom (var: Var): Φ
-| var_is_not_bottom (var: Var): Φ
+| var_is_bottom (var: Var) : Φ
+| var_is_not_bottom (var: Var) : Φ
 | or (ty1: Φ) (ty2: Φ): Φ
 | and (ty1: Φ) (ty2: Φ): Φ
+
 
 -- ## Semantic
 -- This describes the semantic of Refinement Types.
 def Φ_eval: Φ → Env → option Env
 | Φ.false env := none
 | Φ.true env := some env
-| (Φ.xgrd grd) env := xgrd_eval grd env
+| (Φ.xgrd_in grd ty) env := match xgrd_eval grd env with
+    | some env := Φ_eval ty env
+    | none := none
+    end
 | (Φ.not_xgrd grd) env :=
     match xgrd_eval grd env with
     | some env := none
@@ -103,15 +108,29 @@ def Φ_eval: Φ → Env → option Env
     end
 | (Φ.and t1 t2) env :=
     match (Φ_eval t1 env) with
-    -- It is important here to continue with the environment after processing t1!
-    | some env' := Φ_eval t2 env'
+    -- env is not passed down
+    | some _ := Φ_eval t2 env
     | none := none
     end
-    
+
 -- ## Uncovered Refinement Types
 
-def 𝒰_acc : Φ → Gdt → Φ
-| acc (Gdt.leaf _) := Φ.false
+
+-- Alternative definition without accumulator
+def 𝒰' : Gdt → Φ
+| (Gdt.leaf _) := Φ.false
+| (Gdt.branch tr1 tr2) := (𝒰' tr1).and (𝒰' tr2)
+| (Gdt.grd (Grd.bang var) tree) := ((Φ.var_is_not_bottom var).and (𝒰' tree))
+| (Gdt.grd (Grd.xgrd grd) tree) :=
+                (Φ.not_xgrd grd)
+            .or
+                (Φ.xgrd_in grd (𝒰' tree))
+
+def 𝒰 := 𝒰'
+
+/- TODO:
+def 𝒰_acc : Gdt → (Φ → Φ) → Φ → Φ
+| (Gdt.leaf _) f ty := Φ.false
 | acc (Gdt.branch tr1 tr2) := (𝒰_acc (𝒰_acc acc tr1) tr2)
 | acc (Gdt.grd (Grd.bang var) tree) :=
     𝒰_acc (acc.and $ Φ.var_is_not_bottom var) tree
@@ -121,65 +140,70 @@ def 𝒰_acc : Φ → Gdt → Φ
             (𝒰_acc (acc.and (Φ.xgrd grd)) tree)
 
 def 𝒰 : Gdt → Φ := 𝒰_acc Φ.true
+-/
 
-
--- Alternative definition without accumulator
-def 𝒰' : Gdt → Φ
-| (Gdt.leaf _) := Φ.false
-| (Gdt.branch tr1 tr2) := (𝒰' tr1).and (𝒰' tr2)
-| (Gdt.grd (Grd.bang var) tree) := (Φ.var_is_not_bottom var).and (𝒰' tree)
-| (Gdt.grd (Grd.xgrd grd) tree) :=
-                (Φ.not_xgrd grd)
-            .or
-                ((Φ.xgrd grd).and (𝒰' tree))
 
 -- # Annotate
 
-inductive Ant
-| leaf (ty: Φ) (leaf: Leaf): Ant
+inductive Ant (α: Type)
+| leaf (a: α) (leaf: Leaf): Ant
 | branch (tr1: Ant) (tr2: Ant): Ant
-| diverge (ty: Φ) (tr: Ant): Ant
+| diverge (a: α) (tr: Ant): Ant
 
-def 𝒜_acc : Φ → Gdt → Ant
+
+-- Alternative definition without accumulator
+def map_ant { α : Type } { β : Type } : (α → β) → Ant α → Ant β
+| f (Ant.leaf a leaf) := Ant.leaf (f a) leaf
+| f (Ant.branch tr1 tr2) := (Ant.branch (map_ant f tr1) (map_ant f tr2))
+| f (Ant.diverge a tr) := (Ant.diverge (f a) (map_ant f tr))
+
+def 𝒜' : Gdt → Ant Φ
+| (Gdt.leaf leaf) := Ant.leaf Φ.true leaf
+| (Gdt.branch tr1 tr2) := Ant.branch (𝒜' tr1) $ map_ant ((𝒰' tr1).and) (𝒜' tr2)
+| (Gdt.grd (Grd.bang var) tr) := Ant.diverge (Φ.var_is_bottom var) $ map_ant ((Φ.var_is_not_bottom var).and) (𝒜' tr)
+| (Gdt.grd (Grd.xgrd grd) tr) := map_ant (Φ.xgrd_in grd) (𝒜' tr)
+
+def 𝒜 := 𝒜'
+
+/- TODO
+def 𝒜_acc : Φ → Gdt → Ant Φ
 | acc (Gdt.leaf leaf) := Ant.leaf acc leaf
 | acc (Gdt.branch tr1 tr2) := Ant.branch (𝒜_acc acc tr1) (𝒜_acc (𝒰_acc acc tr1) tr2)
 | acc (Gdt.grd (Grd.bang var) tr) := Ant.diverge (acc.and (Φ.var_is_bottom var)) (𝒜_acc (acc.and $ Φ.var_is_not_bottom var) tr)
 | acc (Gdt.grd (Grd.xgrd grd) tr) := (𝒜_acc (acc.and $ Φ.xgrd grd) tr)
 
-def 𝒜 : Gdt → Ant := 𝒜_acc Φ.true
-
+-- wie U[return(Phi) <- Ant Phi]
+def 𝒜 : Gdt → Ant Φ := 𝒜_acc Φ.true
+-/
 
 -- ## Semantics of Ant
 
-inductive AntResult
-| leaf (leaf: Leaf): AntResult
-| diverged : AntResult
+def ant_eval_all (ant: Ant Φ) (env: Env) := map_ant (λ ty, Φ_eval ty env) ant
 
-def ant_eval_list : Ant → Env → list AntResult
-| (Ant.leaf ty leaf) env := match Φ_eval ty env with
-    | none := []
-    | (some env) := [AntResult.leaf leaf]
+def ant_eval' : Ant (option Env) → option Result
+| (Ant.leaf env leaf) := match env with
+    | some env := some $ Result.leaf leaf
+    | none := some $ Result.no_match
     end
-| (Ant.branch tr1 tr2) env := (ant_eval_list tr1 env) ++ (ant_eval_list tr2 env)
-| (Ant.diverge diverge_ty tr) env := match Φ_eval diverge_ty env with
-    | none := ant_eval_list tr env
-    | (some env) := [AntResult.diverged]
+| (Ant.branch tr1 tr2) :=  match (ant_eval' tr1, ant_eval' tr2) with
+    | (some no_match, r) := r
+    | (r, some no_match) := r
+    | _ := none
     end
-
-def ant_eval (tree: Ant) (env: Env) : option Result :=
-    match ant_eval_list tree env with
-    | (AntResult.leaf leaf) :: [] := some (Result.leaf leaf)
-    | (AntResult.diverged) :: [] := some Result.diverged
+| (Ant.diverge env tr) := match (env, ant_eval' tr) with
+    | (none, r) := r
+    | (some env, some Result.no_match) := some Result.diverged
     | _ := none
     end
 
-def result_to_list { α: Type _ } : option α → list α
-| none := []
-| (some val) := [val]
+def ant_eval (ant: Ant Φ) (env: Env): option Result := ant_eval' (ant_eval_all ant env)
+
+
 
 variable is_empty: Φ → bool
 
-def ℛ : Ant → list Leaf × list Leaf × list Leaf
+-- returns (accessible, inaccessible, redundant) leaves, given that `is_empty` is correct.
+def ℛ : Ant Φ → list Leaf × list Leaf × list Leaf
 | (Ant.leaf ty n) := if is_empty ty then ([], [], [n]) else ([n], [], [])
 | (Ant.diverge ty tr) := 
     match (ℛ tr, is_empty ty) with
@@ -226,4 +250,4 @@ def remove_leaves [decidable_eq Leaf] : list Leaf → Gdt → option Gdt
 -- This accounts for empty guard trees.
 def gdt_eval_option : option Gdt → Env → Result
 | (some gdt) env := gdt_eval gdt env
-| none env := Result.no_match env
+| none env := Result.no_match
